src/Actions/FunctionAction.dfy
@@ -17,50 +17,47 @@ module Functions {
       reads this, Repr 
       ensures Valid() ==> this in Repr 
       ensures Valid() ==> 
-        && CanProduce(consumed, produced)
+        && CanProduce(history)
       decreases height, 0
     {
       && this in Repr
-      && CanProduce(consumed, produced)
-      && produced == Seq.Map(f, consumed)
+      && CanProduce(history)
+      && Produced() == Seq.Map(f, Consumed())
     }
 
     constructor(f: T -> R) 
       ensures Valid()
       ensures this.f == f
       ensures fresh(Repr)
-      ensures consumed == []
+      ensures history == []
     { 
       this.f := f;
 
-      consumed := [];
-      produced := [];
+      history := [];
       Repr := {this};
     }
 
-    ghost predicate CanConsume(consumed: seq<T>, produced: seq<R>, next: T)
-      requires CanProduce(consumed, produced)
+    ghost predicate CanConsume(history: seq<(T, R)>, next: T)
+      requires CanProduce(history)
       decreases height
     {
       f.requires(next)
     }
-    ghost predicate CanProduce(consumed: seq<T>, produced: seq<R>)
+    ghost predicate CanProduce(history: seq<(T, R)>)
       decreases height
     {
-      && (forall t <- consumed :: f.requires(t))
-      && produced == Seq.Map(f, consumed)
+      forall e <- history :: f.requires(e.0) && e.1 == f(e.0)
     }
 
     method Invoke(t: T) returns (r: R) 
-      requires Valid()
-      requires CanConsume(consumed, produced, t)
-      modifies Repr
-      decreases height
-      ensures Valid()
-      ensures fresh(Repr - old(Repr))
-      ensures consumed == old(consumed) + [t]
-      ensures produced == old(produced) + [r]
+      requires Requires(t)
+      reads Reads(t)
+      modifies Modifies(t)
+      decreases Decreases(t).Ordinal()
+      ensures Ensures(t, r)
+      ensures EnsuresTwostate(t)
     {
+      assert Valid();
       r := f(t);
 
       Update(t, r);
@@ -70,11 +67,10 @@ module Functions {
   method Example() {
     var doubler := new FunctionAction(v => v + v);
     
-    assert doubler.consumed == [];
-    assert doubler.produced == [];
+    assert doubler.history == [];
     
     var x := doubler.Invoke(2);
-    assert doubler.produced == [x];
+    assert doubler.Produced() == [x];
     assert [x] == [4];
     assert x == 4;
   }
